# CIS\*4720 Image Processing and Vision

## Assignment 2 Part 1 & 2

### Maneesh Wijewardhana (1125828)

I have read and understood the Academic Misconduct section in the course outline. I assert this work is my own.

**1a)**

-   Let $h = G_1 + G_2$ which by definition, is infinite

-   Then for any $(x,y) \in 0..M-1 \to 0..N-1$ we have

    -   $T_f(h)(x,y) = \sum^{m-1}_{u=0}\sum^{n-1}_{v=0}f(u,v)h(x+u-\frac{m-1}{2}, y+v-\frac{n-1}{2})$

    -   $= \sum^{m-1}_{u=0}\sum^{n-1}_{v=0}f(u,v)(G_1(x+u-\frac{m-1}{2}, y+v-\frac{n-1}{2}) + G_2(x+u-\frac{m-1}{2}, y+v-\frac{n-1}{2}))$

    -   Then by distributing the sum over addition we get:

    -   $= \sum^{m-1}_{u=0}\sum^{n-1}_{v=0}f(u,v)(G_1(x+u-\frac{m-1}{2}, y+v-\frac{n-1}{2}) + f(u,v)G_2(x+u-\frac{m-1}{2}, y+v-\frac{n-1}{2}))$

    -   $= \sum^{m-1}_{u=0}\sum^{n-1}_{v=0}f(u,v)G_1(x+u-\frac{m-1}{2}, y+v-\frac{n-1}{2}) + \sum^{m-1}_{u=0}\sum^{n-1}_{v=0}f(u,v)G_2(x+u-\frac{m-1}{2}, y+v-\frac{n-1}{2})$

    -   $= T_f(G_1)(x,y) + T_f(G_2)(x,y)$

    -   $\therefore T_f(G_1+G_2) = T_f(G_1) + T_f(G_2)$

**1b)**

-   Consider a zero padded infinite image $G_1 = \begin{bmatrix}
3 & 9 & 5\\
3 & 3 & 6\\
4 & 5 & 3
\end{bmatrix} \land G_2 = \begin{bmatrix}8 & 6 & 9 \\ 3 & 10 & 15 \\  6 & 1 & 20 \end{bmatrix}$

-   Consider the neighborhood $f = \begin{bmatrix} 0 & 1 & 0 \\ 1 & 0 & 1 \\ 0 & 1 & 0  \end{bmatrix}$

    -   $\therefore S_f\{(0, 1), (1, 0), (1, 2), (2, 1)\}$

-   Then $G_1 + G_2 = \begin{bmatrix}11 & 15 & 14\\ 6 & 13 & 21\\10 & 6 & 23  \end{bmatrix}$

-   When we apply our neighborhood $f$, we get the set $MIN_f(G_1+G_2)\{15, 6, 21, 6\} = \bold{6}$

-   When we calculate $MIN_f(G_1) + MIN_f(G_2)$, we get $3+1=\bold4$

-   $\therefore MIN_f(G_1+G_2) \ne MIN_f(G_1)+MIN_f(G_2)$ due to a counterexample

**1c)**

-   Consider the same zero padded infinite images and neighborhood defined in **1b)**

-   When we apply our neighborhood $f$, we get the set $MED_f(G_1+G_2)\{6, 6, 15, 21\} = \bold{13.5}$

-   When we calculate $MED_f(G_1) + MED_f(G_2)$, we get $5.5+4.5=\bold{10}$

-   $\therefore MED_f(G_1+G_2) \ne MED_f(G_1)+MED_f(G_2)$ due to a counterexample

**1d)**

-   Consider the same zero padded infinite images and neighborhood defined in **1b)**

-   When we apply our neighborhood $f$, we get the set $MAX_f(G_1+G_2)\{15, 6, 21, 6\} = \bold{21}$

-   When we calculate $MAX_f(G_1) + MAX_f(G_2)$, we get $9+15=\bold{24}$

-   $\therefore MAX_f(G_1+G_2) \ne MAX_f(G_1)+MAX_f(G_2)$ due to a counterexample

**2a)**

-   Let's consider the case where $k = 0$, then $T_f(k*G)(x,y) = \sum^{m-1}_{u=0} \sum^{n-1}_{v=0} f(u,v)(k*G)(x+u-\frac{m-1}{2}, y+v-\frac{n-1}{2}) = 0 \; \forall (x,y) \in 0..M-1 \times 0..N-1$ since $k*G$ is zero everywhere

-   Similarly, $k*T_f(G)(x,y) = k\sum^{m-1}_{u=0}\sum^{n-1}_{v=0}f(u,v)G(x+u-\frac{m-1}{2}, y+v-\frac{n-1}{2}) = 0 \; \forall (x,y) \in 0..M-1 \times 0..N-1$ since $k$ is zero

-   $\therefore T_f(k*G) = k * T_f(G)$ holds when $k = 0$

-   Now let's consider the case where k is not zero, then we have:

    -   $T_f(k*G)(x,y) = \sum^{m-1}_{u=0}\sum^{n-1}_{v=0}f(u,v)(k*G)(x+u-\frac{m-1}{2}, y+v-\frac{n-1}{2})$ **(factor)**

    -   $= k \sum^{m-1}_{u=0}\sum^{n-1}_{v=0}f(u,v)G(x+u-\frac{m-1}{2}, y+v-\frac{n-1}{2})$

    -   $= k*T_f(G)(x,y)$

-   $\therefore$ we have proven that $T_f(k*G) = k * T_f(G)$

**2b)**

-   Consider a zero padded infinite image $G = \begin{bmatrix}
3 & 9 & 5\\
3 & 3 & 6\\
4 & 5 & 3
\end{bmatrix}$

-   Consider the neighborhood $f = \begin{bmatrix} 0 & 1 & 0 \\ 1 & 0 & 1 \\ 0 & 1 & 0  \end{bmatrix}$

    -   $\therefore S_f\{(0, 1), (1, 0), (1, 2), (2, 1)\}$

-   When we apply our neighborhood $f$, we get the set $MIN_f(k*G)\{-27, -9, -18, -15\} = \bold{-27}$

-   When we calculate $k * MIN_f(G)$, we get $(-3)*3=\bold{-9}$

-   $\therefore MIN_f(k*G) \ne k* MIN_f(G)$ due to a counterexample

**2c)**

-   We have $G(x+u-\frac{m-1}{2}, y+v-\frac{n-1}{2})$

-   We need to show that multiplying all the values by $k$ does not change the number of values below or above the median
-   Let's consider the set of values below the median of the unscaled values, suppose this set has $m$ values
-   Then, the set of scaled values below the median is:
    -   $k*G(x+u-\frac{m-1}{2}, y+v-\frac{n-1}{2})$ for $(u,v) \in S_f$, sorted in increasing order where there are $m$ values in this set
-   Multiplying all these values by $k$ does not change their order, so the value that was previously the median of the unscaled values is now the $(m/2)$-th largest value in the scaled set
-   $\therefore$ the number of values below the median is still $m$, and the number of values above the median is still the same as well
-   The same argument applies to the set of values above the median, so the number of values below and above the median is unchanged when we scale the values by $k$
-   $\therefore$ we have shown that $MED_f(k*G) = k*MED_f(G)$

**2d)**

-   Consider the same zero padded infinite images and neighborhood defined in **2b)**

-   When we apply our neighborhood $f$, we get the set $MAX_f(k*G)\{-27, -9, -18, -15\} = \bold{-9}$
-   When we calculate $k * MAX_f(G)$, we get $(-3)*(-9)=\bold{27}$
-   $\therefore MAX_f(k*G) \ne k* MAX_f(G)$ due to a counterexample

**3a)**

-   Since $F(x,y) = 0 \; \forall (x,y) \in \mathbb{Z}^2$, any infinite image $G$ where $G \; R \; F$ must satisfy $G(x+a,y+b) = 0 \; \forall (x,y)$ and some $(a,b) \in \mathbb{Z}^2$

-   This means that $G(x,y)$ must also equal to 0 $\forall (x,y) \in \mathbb{Z}^2$
-   $\therefore$ there is only one infinite image that is related to $F$, more specifically, the function $G(x,y) = 0 \; \forall (x,y) \in \mathbb{Z}^2$

**3b)**

-   Let $H$ be an infinite image where $H \; R \; G$

-   Then $\exists$ a pair of integers $(a,b) \; | \; \forall (x,y) \in \mathbb{Z}^2, H(x+a,y+b)=G(x,y)$. In particular, we have $H(a,b) = G(0,0) = 1$
-   If we consider the values of $H$ in the first row $(y=0)$ and the first column $(x=0)$, we have:
    -   $H(x+a,b) = G(x,0) = 0 \; \forall x \ne0$

    -   $H(a, y+b) = G(0,y) = 0 \; \forall y \ne0$
-   $\therefore H$ must be constant along each row and each column, with the value of 0 everywhere except for $H(a,b) = 1$
-   This means that any infinite image like above is related to $G$
-   $\therefore$ the number of infinite images that are related to $G$ is the same as the number of choices for the cell $(a,b)$ which is infinite since $\mathbb{Z}^2$ is infinite

**3c)**

-   Consider the infinite image $H$ defined as follows:

    -   $H(x,y) = 0$ if $(x,y) \in \{(2n, 2m) | n, m \in \mathbb{Z}\}$ (i.e, $H$ is 0 at all even coordinates)

    -   $H(x,y) = 1$ if $(x,y) \in \{(2n+1, 2m+1) | n, m \in \mathbb{Z}\}$ (i.e, $H$ is 1 at all odd coordinates)
-   We claim that H is related to exactly $F \land G$
-   To see this, note that for any $(x,y) \in \mathbb{Z}^2$, either $(x,y)$ is even or odd
    -   If $(x,y)$ is even:
        -   $(x-2n, y-2m)$ is also even for any $(n,m) \in \mathbb{Z}^2$

        -   $\therefore$ for any $(a,b) \in \mathbb{Z}^2$ we have $H(x+a, y+b) = 0 = F(x+a-a, y+b-b)$
    -   If $(x,y)$ is odd:
        -   $(x-2n-1, y-2m-1)$ is also odd for any $(n,m) \in \mathbb{Z}^2$

        -   $\therefore$ for any $(a,b) \in \mathbb{Z}^2$ we have $H(x+a, y+b) = 1 = G(x+a-a, y+b-b)$
-   Thus, $H$ is related to both $F \land G$
-   To show that $H$ is not realted to any other infinite image, let's take another image $K$ such that $H \; R \; K$
-   This means $H(x+a, y+b) = K(x,y)$
-   Consider the case where $(a,b) = (0, 0)$, then $\forall (x,y) \in \mathbb{Z}^2$ we have $H(x,y) = K(x,y)$
-   In particular, this implies that for all odd $(x,y) \in \mathbb{Z}^2, K(x,y) = 1$ and for all even $(x,y) \in \mathbb{Z}^2, K(x,y) = 0$
-   However, this means that $K$ has the same pattern as $G$ which we have already shown is related to $H$

**4a)**

-   $f^C$ can be formally defined as follows:

    -   $\forall(x,y) \in 0..M-1 \times 0..N-1, f^C(x,y)=f(x,y)$

    -   $\forall(x,y) \notin 0..M-1 \times 0..N-1, \forall(i,j) \in \mathbb{Z}^2, f^C(x + iM, y+ jN) = f(x,y)$

**4b)**

-   $f^R$ can be formally defined as follows:

    -   $f^R(x,y) = f(|x'|, |y'|)$ where $x' \land y'$ are defined as follows:

        -   $x' = x$ if $0\le x < M$

        -   $x' = -x$ if $-M \le x < 0$
        -   $x' = 2M - x - 1$ if $x \ge M$
        -   $y' = y$ if $0 \le y < N$
        -   $y' = -y$ if $-N \le y < 0$
        -   $y' = 2N - x - 1$ if $y \ge N$

**5a)**

-   There is only **1** Z-image that are also C-images which is the 0 image

-   $[...0\;0\;0...]$

**5b)**

-   There is only **1** Z-image that are also R-images which is the 0 image

-   $[...0\;0\;0...]$

**5c)**

-   R-images are also C-images due to this concept:

-   If we take an R-image like $[1\;2\;3]^R$, we can expand it out to $[...1\;2\;3\;3\;2\;1\;1\;2\;3...]^R$
-   We can see that in this case, the values $[3 \; 2\;1]$ are seen when $2m\times2n$ which is reflected
-   However, we can also see that the values $[1 \;2\;3]$ are seen when $4m\times4n$ which corresponds to the C-image because the original was $[1\;2\;3]^R$

**5d)**

-   If we take a C-image defined as $[1 \; 2 \; 3]^C$, expanding it out gets us $[1 \; 2 \; 3 \; 1 \; 2 \; 3]^C$ which is not reflected and thus, not an R-image

**6a)**

-   The infinite image that has no discernible patterns such as zero padding, circular indexing, or reflected indexing, but rather consists of random values would allow for no minimum generator

-   For example, if we add 1s in random spots:

    -   $[...1\;3\;1\;1\;2\;1\;1...]$ does not have a minimum generator

    -   The 1 values can be replaced by any integer which would allow for it to be an infinite image

**6b)**

-   An infinite image with 1 value in it would by definition have exactly 1 minimum generator which would be itself

-   For example:
    -   The infinite image $[...1...]^C$

    -   This image has exactly 1 minimum generator defined as $[1]$

**6c)**

-   An infinite image with 2 values repeating would by definition have exactly 2 minimum generators which would be the 2 values in either direction

-   For example:
    -   The infinite image $[...1\;0\;1\;0\;1\;0...]^C$

    -   This image has exactly 2 minimum generators defined as $[1\;0]$ and $[0\;1]$
